\documentclass[12pt]{article}
%\usepackage{ifthen, latexsym, amsfonts}
\usepackage{url,mathtools,color}
\usepackage{amsmath}
\usepackage{ amssymb }

\begin{document}
\title{\large \sc Neher and Leitner Analysis
\\ Elena Romero}
\maketitle
\vskip-10pt

\[P(\text{no AB}) = (1-p_{AB})^M \approx e^{-Mp_{AB}}\]

We can start with our frequency of the AB haplotype, $p_{AB}$ over time.

\begin{equation}
p_{AB}(\Delta t) = p_A p_B + (p_{ab}^0 - p_Ap_B)e^{- \rho d \Delta t}
\end{equation}

\begin{itemize}
\item First we consider the case where $\rho d \Delta t << 1$. We begin by using a taylor's approximation for the $e^x$ term in equation 1. This yields

\[p_{AB}(\Delta t)  \approx p_A p_B + (p_{ab}^0 - p_Ap_B)(1 - \rho d \Delta t)\]
\[p_{AB}(\Delta t)  \approx p_{ab}^0 + (p_Ap_B - p_{ab}^0) \rho d \Delta t\]

Now we can substitute this into 
\[\mathcal{P}(d(t_{i+1}-t_i)) = 1 - e^{-Mp_{AB}{(t_i + 1)}}\]
Which gives us 
\[\mathcal{P}(d(t_{i+1}-t_i)) = 1 - e^{- M(p_{AB}^0 + (p_Ap_B - p_{AB}^0)\rho d \Delta t)}\]
To solve for $\rho$, we need to take the derivative of this with respect to $d \Delta t$. Then we can evaluate this derivative at $d \Delta t = 0$. Once we have this, we can set it equal to $f'(0)$ and solve for $\rho$.

Taking the derivative of $1 - e^{- M(p_{AB}^0 + (p_Ap_B - p_{AB}^0)\rho d \Delta t)}$ with respect to $d\Delta t$ gives us
\[\mathcal{P}'(d \Delta t) = e^{-Mp_{AB}^0}e^{-M(p_Ap_B - p_{AB}^0)\rho d \Delta t}(M(p_Ap_B - p_{AB}^0))\rho\]
Evaluating it at $d \Delta t = 0$ yields
\begin{equation}\mathcal{P}'(d \Delta t) = e^{-Mp_{AB}^0}(M(p_Ap_B - p_{AB}^0))\rho\end{equation}

So, the slope is proportional to $\rho$ at $d \Delta t = 0$. We will fit the curve using the function
\[f(d\Delta t) = c_0 + c_1(1-e^{-c_2d\Delta t})\]
Taking the derivative of our fit function,
\[f'(d\Delta t) = c_1c_2e^{-c_2d\Delta t}\]
Evaluating at $d \Delta t = 0$
\[f'(0) = c_1c_2\]
Now, we can set this expression equal to equation 2, since they are both expressions for the slope at 0, and solve for $\rho$
\[c_1c_2 = \hat{\rho} e^{-Mp_{AB}^0}(M(p_Ap_B - p_{AB}^0))\]
\[\hat{\rho} = \frac{c_1c_2}{e^{-Mp_{AB}^0}(Mp_Ap_B - Mp_{AB}^0)}\]
Lastly, the intercept $\mathcal{P}(0) = 1 - e^{-Mp_{AB}^0} = c_0$, so we can substitute this in to get
\begin{equation}\hat{\rho} = \frac{c_1c_2}{(1-c_0)\left(Mp_Ap_B  - \ln\left(\frac{1}{1- c_0}\right)\right)}\end{equation}
\\
%%%%%%%%%%%%%%%%%%%%% Item 2 %%%%%%%%%%%%%%%%%%%%%%%
\item Next we consider the case where $\rho d \Delta t >> 1$.
In this case, the second term in equation 1 goes to 0 which leaves us with
\[p_{AB}(\Delta t) = p_A p_B\]
Plugging this into 
\[\mathcal{P}(d(t_{i+1}-t_i)) = 1 - e^{-Mp_{AB}{(t_i + 1)}}\]
yields 
\[\mathcal{P}(d(t_{i+1}-t_i)) = 1 - e^{-Mp_Ap_B}\]
As $\rho d \Delta$ goes to $+\infty$ our fit function $f$ goes to 
\[lim_{d \Delta t \rightarrow +\infty}f(d\Delta t) = c_0 + c_1\]
Therefore, for $\rho d \Delta t >> 1$, the curve should eventually saturate to 
\[\mathcal{P}(d(t_{i+1}-t_i)) = 1 - e^{-Mp_Ap_B} =  c_0 + c_1\]
If we solve this for $Mp_Ap_B$, we get
\begin{equation}Mp_Ap_B =  \ln \left(\frac{1}{1 - c_0 - c_1}\right)\end{equation}
\end{itemize}

We can use equations 3 and 4 to get

\[\hat{\rho} = \frac{c_1c_2}{(1-c_0)\left( \ln \left(\frac{1}{1 - c_0 - c_1}\right) - \ln\left(\frac{1}{1- c_0}\right)\right)}\]



\end{document}